deleted the free assume about gates after parallel calls

Test/og/ticket.bpl
@@ -8,10 +8,10 @@ axiom (forall x: int, y: int :: RightClosed(x)[y] <==> y <= x);
 type X;
 function {:builtin "MapConst"} mapconstbool(bool): [X]bool;
 const nil: X;
-var {:phase 3} t: int;
-var {:phase 3} s: int;
-var {:phase 3} cs: X;
-var {:phase 3} T: [int]bool;
+var {:phase 2} t: int;
+var {:phase 2} s: int;
+var {:phase 2} cs: X;
+var {:phase 2} T: [int]bool;
 
 function {:builtin "MapConst"} MapConstBool(bool) : [X]bool;
 function {:inline} {:linear "tid"} TidCollector(x: X) : [X]bool
@@ -36,17 +36,18 @@ function {:inline} Inv2(tickets: [int]bool, ticket: int, lock: X): (bool)
 procedure Allocate({:linear_in "tid"} xls':[X]bool) returns ({:linear "tid"} xls: [X]bool, {:linear "tid"} xl: X);
 ensures {:phase 1} {:phase 2} xl != nil;
 
-procedure {:yields} {:phase 3} main({:linear_in "tid"} xls':[X]bool)
-requires {:phase 3} xls' == mapconstbool(true);
+procedure {:yields} {:phase 2} main({:linear_in "tid"} xls':[X]bool)
+requires {:phase 2} xls' == mapconstbool(true);
 {
     var {:linear "tid"} tid: X;
     var {:linear "tid"} xls: [X]bool;
 
     yield;
 
-    call xls := Init(xls');
+    call Init(xls');
+    xls := xls';
 
-    par Yield1() | Yield2() | Yield();
+    par Yield1() | Yield2();
 
     while (*)
     invariant {:phase 1} Inv1(T, t);
@@ -54,63 +55,59 @@ requires {:phase 3} xls' == mapconstbool(true);
     {
         call xls, tid := Allocate(xls);
         async call Customer(tid);
-    	par Yield1() | Yield2() | Yield();
+    	par Yield1() | Yield2();
     }
-    par Yield1() | Yield2() | Yield();
+    par Yield1() | Yield2();
 }
 
-procedure {:yields} {:phase 3} Customer({:linear_in "tid"} tid': X)
+procedure {:yields} {:phase 2} Customer({:linear_in "tid"} tid: X)
 requires {:phase 1} Inv1(T, t);
-requires {:phase 2} tid' != nil && Inv2(T, s, cs);
-requires {:phase 3} true;
+requires {:phase 2} tid != nil && Inv2(T, s, cs);
 {
-    var {:linear "tid"} tid: X;
-    tid := tid';
-    
-    par Yield1() | Yield2() | Yield();    
+    par Yield1() | Yield2();    
     while (*) 
     invariant {:phase 1} Inv1(T, t);
-    invariant {:phase 2} tid != nil && Inv2(T, s, cs);
+    invariant {:phase 2} Inv2(T, s, cs);
     {
-        call tid := Enter(tid);
+        call Enter(tid);
+        par Yield1() | Yield2() | YieldSpec(tid);
+    	call Leave(tid);
         par Yield1() | Yield2();
-    	call tid := Leave(tid);
-        par Yield1() | Yield2() | Yield();
     }
-    par Yield1() | Yield2() | Yield();
+    par Yield1() | Yield2();
 }
 
-procedure {:yields} {:phase 2,3} Enter({:linear_in "tid"} tid': X) returns ({:linear "tid"} tid: X)
+procedure {:yields} {:phase 2} Enter({:linear "tid"} tid: X)
 requires {:phase 1} Inv1(T, t);
 ensures {:phase 1} Inv1(T,t);
-requires {:phase 2} tid' != nil && Inv2(T, s, cs);
-ensures {:phase 2} tid != nil && Inv2(T, s, cs);
-ensures {:right} |{ A: tid := tid'; havoc t, T; assume tid != nil && cs == nil; cs := tid; return true; }|;
+requires {:phase 2} tid != nil && Inv2(T, s, cs);
+ensures {:phase 2} Inv2(T, s, cs) && cs == tid;
 {
     var m: int;
 
     par Yield1() | Yield2();
-    tid := tid';
-    call tid, m := GetTicketAbstract(tid);
+    call m := GetTicketAbstract(tid);
     par Yield1();
-    call tid := WaitAndEnter(tid, m);
-    par Yield1() | Yield2();
+    call WaitAndEnter(tid, m);
+    par Yield1() | Yield2() | YieldSpec(tid);
 }
 
-procedure {:yields} {:phase 1,2} GetTicketAbstract({:linear_in "tid"} tid': X) returns ({:linear "tid"} tid: X, m: int)
+procedure {:yields} {:phase 1,2} GetTicketAbstract({:linear "tid"} tid: X) returns (m: int)
 requires {:phase 1} Inv1(T, t);
 ensures {:phase 1} Inv1(T, t);
-ensures {:right} |{ A: tid := tid'; havoc m, t; assume !T[m]; T[m] := true; return true; }|;
+ensures {:right} |{ A: havoc m, t; assume !T[m]; T[m] := true; return true; }|;
 {
     par Yield1();
-    tid := tid';
-    call tid, m := GetTicket(tid);
+    call m := GetTicket(tid);
     par Yield1();
 }
 
-procedure {:yields} {:phase 3} Yield()
+procedure {:yields} {:phase 2} YieldSpec({:linear "tid"} tid: X)
+requires {:phase 2} tid != nil && cs == tid;
+ensures {:phase 2} cs == tid;
 {
     yield;
+    assert {:phase 2} tid != nil && cs == tid;
 }
 
 procedure {:yields} {:phase 2} Yield2()
@@ -129,15 +126,15 @@ ensures {:phase 1} Inv1(T,t);
     assert {:phase 1} Inv1(T,t);
 }
 
-procedure {:yields} {:phase 0,3} Init({:linear_in "tid"} xls':[X]bool) returns ({:linear "tid"} xls:[X]bool);
-ensures {:atomic} |{ A: assert xls' == mapconstbool(true); xls := xls'; cs := nil; t := 0; s := 0; T := RightOpen(0); return true; }|;
+procedure {:yields} {:phase 0,2} Init({:linear "tid"} xls:[X]bool);
+ensures {:atomic} |{ A: assert xls == mapconstbool(true); cs := nil; t := 0; s := 0; T := RightOpen(0); return true; }|;
 
-procedure {:yields} {:phase 0,1} GetTicket({:linear_in "tid"} tid': X) returns ({:linear "tid"} tid: X, m: int);
-ensures {:atomic} |{ A: tid := tid'; m := t; t := t + 1; T[m] := true; return true; }|;
+procedure {:yields} {:phase 0,1} GetTicket({:linear "tid"} tid: X) returns (m: int);
+ensures {:atomic} |{ A: m := t; t := t + 1; T[m] := true; return true; }|;
 
-procedure {:yields} {:phase 0,2} WaitAndEnter({:linear_in "tid"} tid': X, m:int) returns ({:linear "tid"} tid: X);
-ensures {:atomic} |{ A: tid := tid'; assume m <= s; cs := tid; return true; }|;
+procedure {:yields} {:phase 0,2} WaitAndEnter({:linear "tid"} tid: X, m:int);
+ensures {:atomic} |{ A: assume m <= s; cs := tid; return true; }|;
 
-procedure {:yields} {:phase 0,3} Leave({:linear_in "tid"} tid': X) returns ({:linear "tid"} tid: X);
-ensures {:atomic} |{ A: assert cs == tid'; assert tid' != nil; tid := tid'; s := s + 1; cs := nil; return true; }|;
+procedure {:yields} {:phase 0,2} Leave({:linear "tid"} tid: X);
+ensures {:atomic} |{ A: s := s + 1; cs := nil; return true; }|;
 
