Test/og/multiset.bpl
@@ -20,92 +20,85 @@ function {:inline} {:linear "tid"} TidCollector(x: X) : [X]bool
 
 axiom (max > 0);
 
-procedure {:yields} {:phase 0} acquire(i : int, {:linear_in "tid"} tidIn: X) returns ({:linear "tid"} tidOut: X);
+procedure {:yields} {:phase 0} acquire(i : int, {:linear "tid"} tid: X);
 ensures {:right} |{ A: 
                       assert 0 <= i && i < max;
-                      assert tidIn != nil && tidIn != done;
+                      assert tid != nil && tid != done;
                       assume lock[i] == nil;
-                      tidOut := tidIn;
-	              lock[i] := tidOut;
+	              lock[i] := tid;
                       return true;
                     }|;
 
 
-procedure {:yields} {:phase 0} release(i : int, {:linear_in "tid"} tidIn: X) returns ({:linear "tid"} tidOut: X);
+procedure {:yields} {:phase 0} release(i : int, {:linear "tid"} tid: X);
 ensures {:left} |{ A: 
                      assert 0 <= i && i < max;
-                     assert lock[i] == tidIn;
-                     assert tidIn != nil && tidIn != done; 
-                     tidOut := tidIn;
+                     assert lock[i] == tid;
+                     assert tid != nil && tid != done; 
 	             lock[i] := nil;
                      return true;
                     }|;
 
 
-procedure {:yields} {:phase 0,1} getElt(j : int, {:linear_in "tid"} tidIn: X) returns ({:linear "tid"} tidOut: X, elt_j:int);
+procedure {:yields} {:phase 0,1} getElt(j : int, {:linear "tid"} tid: X) returns (elt_j:int);
 ensures {:both} |{ A: 
                      assert 0 <= j && j < max;
-                     assert lock[j] == tidIn;
-                     assert tidIn != nil && tidIn != done;
-                     tidOut := tidIn;
+                     assert lock[j] == tid;
+                     assert tid != nil && tid != done;
 	             elt_j := elt[j];
                      return true;
                     }|;
 
 
-procedure {:yields} {:phase 0,1} setElt(j : int, x : int, {:linear_in "tid"} tidIn: X) returns ({:linear "tid"} tidOut: X);
+procedure {:yields} {:phase 0,1} setElt(j : int, x : int, {:linear "tid"} tid: X);
 ensures {:both} |{ A: 
                      assert x != null;
                      assert owner[j] == nil;
                      assert 0 <= j && j < max;
-                     assert lock[j] == tidIn;
-                     assert tidIn != nil && tidIn != done;
-                     tidOut := tidIn;
+                     assert lock[j] == tid;
+                     assert tid != nil && tid != done;
 	             elt[j] := x;
-                     owner[j] := tidIn;
+                     owner[j] := tid;
                      return true;
                     }|;
 
 
-procedure {:yields} {:phase 0} setEltToNull(j : int, {:linear_in "tid"} tidIn: X) returns ({:linear "tid"} tidOut: X);
+procedure {:yields} {:phase 0} setEltToNull(j : int, {:linear "tid"} tid: X);
 ensures {:left} |{ A: 
-                     assert owner[j] == tidIn;
+                     assert owner[j] == tid;
                      assert 0 <= j && j < max;
-                     assert lock[j] == tidIn;
+                     assert lock[j] == tid;
                      assert !valid[j];
-                     assert tidIn != nil  && tidIn != done;
-                     tidOut := tidIn;
+                     assert tid != nil  && tid != done;
 	             elt[j] := null;
                      owner[j] := nil;
                      return true;
                     }|;
 
-procedure {:yields} {:phase 0} setValid(j : int, {:linear_in "tid"} tidIn: X) returns ({:linear "tid"} tidOut: X);
+procedure {:yields} {:phase 0} setValid(j : int, {:linear "tid"} tid: X);
 ensures {:both} |{ A: 
                      assert 0 <= j && j < max;
-                     assert lock[j] == tidIn;
-                     assert tidIn != nil && tidIn != done;
-                     assert owner[j] == tidIn;
-                     tidOut := tidIn;
+                     assert lock[j] == tid;
+                     assert tid != nil && tid != done;
+                     assert owner[j] == tid;
 	             valid[j] := true;
                      owner[j] := done;
                      return true;
                     }|;
 
-procedure {:yields} {:phase 0} isEltThereAndValid(j : int, x : int, {:linear_in "tid"} tidIn: X) returns ({:linear "tid"} tidOut: X, fnd:bool);
+procedure {:yields} {:phase 0} isEltThereAndValid(j : int, x : int, {:linear "tid"} tid: X) returns (fnd:bool);
 ensures {:both} |{ A: 
                        assert 0 <= j && j < max;
-                       assert lock[j] == tidIn;
-                       assert tidIn != nil && tidIn != done;
-                       tidOut := tidIn;
+                       assert lock[j] == tid;
+                       assert tid != nil && tid != done;
                        fnd := (elt[j] == x) && valid[j];
                        return true;
                     }|;
 
-procedure {:yields} {:phase 1} FindSlot(x : int, {:linear_in "tid"} tidIn: X) returns (r : int, {:linear "tid"} tidOut: X)
-requires {:phase 1} Inv(valid, elt, owner);
+procedure {:yields} {:phase 1} FindSlot(x : int, {:linear "tid"} tid: X) returns (r : int)
+requires {:phase 1} Inv(valid, elt, owner) && x != null && tid != nil && tid != done; 
 ensures {:phase 1} Inv(valid, elt, owner);
-ensures {:right}  |{ A: assert tidIn != nil && tidIn != done; 
+ensures {:right}  |{   A: assert tid != nil && tid != done; 
                           assert x != null; 
 			  goto B, C;
                        B: assume (0 <= r && r < max); 
@@ -113,112 +106,91 @@ ensures {:right}  |{ A: assert tidIn != nil && tidIn != done;
                                             assume owner[r] == nil;
 					    assume !valid[r];
                                             elt[r] := x; 
-                                            owner[r] := tidIn;
-                                            tidOut := tidIn; 
+                                            owner[r] := tid;
                                             return true;
-                       C: assume (r == -1); tidOut := tidIn; return true; 
+                       C: assume (r == -1); return true; 
                    }|;
 {
 	var j : int;
 	var elt_j : int;
-        var {:linear "tid"} tidTmp: X;
         
         par Yield1();
 
 	j := 0;
-        tidTmp := tidIn;
-
-	
 	while(j < max)
-        invariant {:phase 1} tidTmp != nil && tidTmp != done;
-        invariant {:phase 1} tidTmp == tidIn;
         invariant {:phase 1} Inv(valid, elt, owner);
 	invariant {:phase 1} 0 <= j;
 	{
-                call tidTmp := acquire(j, tidTmp);
-                call tidTmp, elt_j := getElt(j, tidTmp);
+                call acquire(j, tid);
+                call elt_j := getElt(j, tid);
 		if(elt_j == null)
 		{
-                        call tidTmp := setElt(j, x, tidTmp);
-			call tidTmp := release(j, tidTmp);
+                        call setElt(j, x, tid);
+			call release(j, tid);
 			r := j;
-                        tidOut := tidTmp;
 
                         par Yield1();
 			return;		
 		}
-		call tidTmp := release(j,tidTmp);
+		call release(j,tid);
 
                 par Yield1();
 
 		j := j + 1;	
 	}
 	r := -1;
-        tidOut := tidTmp;
 
         par Yield1();
 	return;
 }
 
-procedure {:yields} {:phase 2} Insert(x : int, {:linear_in "tid"} tidIn: X) returns (result : bool, {:linear "tid"} tidOut: X) 
-requires {:phase 1} Inv(valid, elt, owner);
-requires {:phase 2} Inv(valid, elt, owner);
+procedure {:yields} {:phase 2} Insert(x : int, {:linear "tid"} tid: X) returns (result : bool) 
+requires {:phase 1} Inv(valid, elt, owner) && x != null && tid != nil && tid != done; 
 ensures {:phase 1} Inv(valid, elt, owner);
-requires {:phase 2} Inv(valid, elt, owner);
+requires {:phase 2} Inv(valid, elt, owner) && x != null && tid != nil && tid != done; 
+ensures {:phase 2} Inv(valid, elt, owner);
 ensures {:atomic}  |{ var r:int;
-                        A: assert tidIn != nil && tidIn != done; 
-                           assert x != null;
-                           goto B, C;
+                        A: goto B, C;
                         B: assume (0 <= r && r < max); 
                            assume valid[r] == false; 
                            assume elt[r] == null; 
                            assume owner[r] == nil; 
                            elt[r] := x; valid[r] := true; owner[r] := done;
-                           tidOut := tidIn; result := true; return true;
-                        C: tidOut := tidIn; result := false; return true; 
+                           result := true; return true;
+                        C: result := false; return true; 
                       }|;
  {
         var i: int;
-        var {:linear "tid"} tidTmp: X;
         par Yield12();
-        tidTmp := tidIn;
-        call i, tidTmp := FindSlot(x, tidTmp);
+        call i := FindSlot(x, tid);
         
 	if(i == -1)
 	{
 		result := false;
-                tidOut := tidTmp;
                 par Yield12();
 		return;
 	}
         par Yield1();
         assert {:phase 1} i != -1;
         assert {:phase 2} i != -1;
-	call tidTmp := acquire(i, tidTmp);
+	call acquire(i, tid);
         assert {:phase 2} elt[i] == x;
 	assert {:phase 2}  valid[i] == false;
-        call tidTmp := setValid(i, tidTmp);   
-	call tidTmp := release(i, tidTmp);
+        call setValid(i, tid);   
+	call release(i, tid);
 	result := true; 
-        tidOut := tidTmp;
         par Yield12();
 	return;
 }
 
-procedure {:yields} {:phase 2} InsertPair(x : int, 
-                               y : int, 
-                               {:linear_in "tid"} tidIn: X) 
-                               returns (result : bool, 
-                                        {:linear "tid"} tidOut: X) 
-requires {:phase 1} Inv(valid, elt, owner);
+procedure {:yields} {:phase 2} InsertPair(x : int, y : int, {:linear "tid"} tid: X) returns (result : bool)
+requires {:phase 1} Inv(valid, elt, owner) && x != null && y != null && tid != nil && tid != done; 
 ensures {:phase 1} Inv(valid, elt, owner);
-requires {:phase 2} Inv(valid, elt, owner);
+requires {:phase 2} Inv(valid, elt, owner) && x != null && y != null && tid != nil && tid != done; 
 ensures {:phase 2} Inv(valid, elt, owner);
 ensures {:atomic}  |{ var rx:int;
                         var ry:int;
-                        A: assert tidIn != nil && tidIn != done; 
-                           assert x != null && y != null;
-                           goto B, C;
+                        A: goto B, C;
                         B: assume (0 <= rx && rx < max && 0 <= ry && ry < max && rx != ry); 
                            assume valid[rx] == false; 
                            assume valid[ry] == false; 
@@ -230,68 +202,60 @@ ensures {:atomic}  |{ var rx:int;
                            valid[ry] := true;
                            owner[rx] := done;
                            owner[ry] := done; 
-                           tidOut := tidIn; 
                            result := true; return true;
-                        C: tidOut := tidIn; 
-                           result := false; return true; 
+                        C: result := false; return true; 
                       }|;
  {
         var i : int; 
         var j : int;
-        var {:linear "tid"} tidTmp: X;
         par Yield12();
 
-        tidTmp := tidIn;
-
-        call i, tidTmp := FindSlot(x, tidTmp);
+        call i := FindSlot(x, tid);
         
 	if (i == -1)
 	{
 	 	result := false;
-                tidOut := tidTmp;
                 par Yield12();
 		return;
 	}
 
         par Yield1();
-        call j, tidTmp := FindSlot(y, tidTmp);
+        call j := FindSlot(y, tid);
         
 	if(j == -1)
 	{
                 par Yield1();
-                call tidTmp := acquire(i,tidTmp);  
-                call tidTmp := setEltToNull(i, tidTmp);
-                call tidTmp := release(i,tidTmp);  
+                call acquire(i,tid);  
+                call setEltToNull(i, tid);
+                call release(i,tid);  
 		result := false;
-                tidOut := tidTmp;
                 par Yield12();
 		return;
 	}
 
         par Yield1();
         assert {:phase 2} i != -1 && j != -1;
-	call tidTmp := acquire(i, tidTmp);
-	call tidTmp := acquire(j, tidTmp);
+	call acquire(i, tid);
+	call acquire(j, tid);
         assert {:phase 2} elt[i] == x;
         assert {:phase 2} elt[j] == y;
 	assert {:phase 2}  valid[i] == false;
 	assert {:phase 2}  valid[j] == false;
-        call tidTmp := setValid(i, tidTmp);   
-        call tidTmp := setValid(j, tidTmp);   
-	call tidTmp := release(j, tidTmp);
-	call tidTmp := release(i, tidTmp);
+        call setValid(i, tid);   
+        call setValid(j, tid);   
+	call release(j, tid);
+	call release(i, tid);
 	result := true; 
-        tidOut := tidTmp;
         par Yield12();
 	return;
 }
 
-procedure {:yields} {:phase 2} LookUp(x : int, {:linear_in "tid"} tidIn: X, old_valid:[int]bool, old_elt:[int]int) returns (found : bool, {:linear "tid"} tidOut: X)
+procedure {:yields} {:phase 2} LookUp(x : int, {:linear "tid"} tid: X, old_valid:[int]bool, old_elt:[int]int) returns (found : bool)
 requires {:phase 1} {:phase 2} old_valid == valid && old_elt == elt;
 requires {:phase 1} {:phase 2} Inv(valid, elt, owner);
-requires {:phase 1} {:phase 2} (tidIn != nil && tidIn != done);
+requires {:phase 1} {:phase 2} (tid != nil && tid != done);
 ensures {:phase 1} {:phase 2} Inv(valid, elt, owner);
-ensures {:atomic}  |{ A: assert tidIn != nil && tidIn != done; 
+ensures {:atomic}  |{ A: assert tid != nil && tid != done; 
                           assert x != null;
                           assume found ==> (exists ii:int :: 0 <= ii && ii < max && valid[ii] && elt[ii] == x);
 			  assume !found ==> (forall ii:int :: 0 <= ii && ii < max ==> !(old_valid[ii] && old_elt[ii] == x));
@@ -300,37 +264,31 @@ ensures {:atomic}  |{ A: assert tidIn != nil && tidIn != done;
 {
 	var j : int;
 	var isThere : bool;
-        var {:linear "tid"} tidTmp: X;
         
         par Yield12() | YieldLookUp(old_valid, old_elt);
 
 	j := 0;
-        tidTmp := tidIn;
 
 	while(j < max)
-        invariant {:phase 1} {:phase 2} tidTmp != nil && tidTmp != done;
-        invariant {:phase 1} {:phase 2} tidTmp == tidIn;
         invariant {:phase 1} {:phase 2} Inv(valid, elt, owner);
         invariant {:phase 1} {:phase 2} (forall ii:int :: 0 <= ii && ii < j ==> !(old_valid[ii] && old_elt[ii] == x));
 	invariant {:phase 1} {:phase 2} (forall ii:int :: 0 <= ii && ii < max && old_valid[ii] ==> valid[ii] && old_elt[ii] == elt[ii]);
 	invariant {:phase 1} {:phase 2} 0 <= j;
 	{
-                call tidTmp := acquire(j, tidTmp);
-                call tidTmp, isThere := isEltThereAndValid(j, x, tidTmp);
+                call acquire(j, tid);
+                call isThere := isEltThereAndValid(j, x, tid);
 		if(isThere)
 		{
-			 call tidTmp := release(j, tidTmp);
+			 call release(j, tid);
                          found := true; 
-                         tidOut := tidTmp;
                          par Yield12() | YieldLookUp(old_valid, old_elt);
 		 	 return;		
 		}
-		call tidTmp := release(j,tidTmp);
+		call release(j,tid);
                 par Yield12() | YieldLookUp(old_valid, old_elt);
 		j := j + 1;	
 	}
 	found := false;
-        tidOut := tidTmp;
 
         par Yield12() | YieldLookUp(old_valid, old_elt);
 	return;
